starting with a few harder rules

theories/Subst.v
@@ -9,6 +9,7 @@ Definition subst_str (x y z : string) := if eqb z x then y else z.
 Arguments subst_str x y/ z.
 Hint Unfold subst_str : core.
 
+(* subst_var e x y = e[x/y]. y goes away, x takes its place. *)
 (* TODO: Joe, please tell me if this is what you had in mind; I guessed from the type signature *)
 Fixpoint subst_var (e : term) (x : string) (y : string) : term :=
   match e with
@@ -17,11 +18,9 @@ Fixpoint subst_var (e : term) (x : string) (y : string) : term :=
       e
   | TmVar z =>
       TmVar (if eqb z y then x else z)
-  | TmComma lhs rhs =>
-      TmComma (subst_var lhs x y) (subst_var rhs x y)
-  | TmSemic lhs rhs =>
-      TmSemic (subst_var lhs x y) (subst_var rhs x y)
-  | TmLet x' e e' => TmLet x' (subst_var e x y) (subst_var e' x y)
+  | TmComma lhs rhs => TmComma (subst_var lhs x y) (subst_var rhs x y)
+  | TmSemic lhs rhs => TmSemic (subst_var lhs x y) (subst_var rhs x y)
+  | TmLet x' e e' => TmLet x' (if eqb y x' then e else subst_var e x y) (subst_var e' x y)
       (* let subst_bound := subst_var bound x y in *)
       (* let subst_body := if eqb bind x then shadowing body else no shadowing subst_var body x y in *)
       (* TmLet bind subst_bound subst_body *)
@@ -36,12 +35,40 @@ Fixpoint subst_var (e : term) (x : string) (y : string) : term :=
   | TmInl e => TmInl (subst_var e x y)
   | TmInr e => TmInr (subst_var e x y)
   | TmPlusCase eta r z x' e1 y' e2 => TmPlusCase eta r z x' (subst_var e1 x y) y' (subst_var e2 x y)
-  end.
+  | TmFix args g r e => TmFix (subst_var_argsterm args x y) g r e
+  | TmRec args => TmRec (subst_var_argsterm args x y)
+  end
+with
+subst_var_argsterm (args : argsterm) (x : string) (y : string) :=
+    match args with
+    | ATmEmpty => ATmEmpty
+    | ATmSng e => ATmSng (subst_var e x y)
+    | ATmComma e1 e2 => ATmComma (subst_var_argsterm e1 x y) (subst_var_argsterm e2 x y)
+    | ATmSemic e1 e2 => ATmSemic (subst_var_argsterm e1 x y) (subst_var_argsterm e2 x y)
+    end
+.
+
 Arguments subst_var e/ x y.
 
-
 (* TODO: will. *)
-Theorem subst_not_fv : forall e x y,
-    ~(fv e y) -> e = subst_var e x y.
+Theorem subst_not_fv : 
+    (forall e, forall x y, ~(fv e y) -> e = subst_var e x y)
+    /\
+    (forall args, forall x y, ~(fv args y) -> args = subst_var_argsterm args x y).
 Proof.
+apply term_mutual; intros.
+- hauto lq: on rew: off.
+- hauto lq: on rew: off.
+- admit.
+- qauto l: on.
+- hauto lq: on rew: off.
+- assert (subst_var (TmLet bind bound body) x y = TmLet bind (if eqb bind y then bound else subst_var bound x y) (subst_var body x y)) by best.
+  rewrite -> H2.
+  cbn in H1.
+  assert (~ fv bound y) by best.
+  assert (~ (fv body y /\ bind <> y)) by best.
+  assert ((~ fv body y) \/ bind = y) by admit.
+  destruct H5.
+  + best.
+  + rewrite -> H5. admit.
 Admitted.
